####According to **ERRATA TO VOLUME 1 (UNTIL 2010)**:

  - Errors:

    **Page 505** second display in answer **9** (17 Oct 2007) [*](#note1):<a id="err1"></a>

    - Before: x^\{z\}
    - (Not modified yet) Should be: x^\{x\}

####According to **ERRATA TO VOLUME 1 (AFTER 2010)**:

  - Amendments:

    **Page 476** replacement for answer **4** (22 Dec 2013):

    - Before: **4.** $x-1\\lt\\lfloor\{x\}\\rfloor≤x$; so $-x+1\\gt-\\lfloor\{x\}\\rfloor≥-x$; hence the result.
    - Actual: **4.** By part (f), $x\\le\\lceil\{x\}\\rceil\\lt x+1$; hence $-x-1\\lt\\lceil\{x\}\\rceil\\le-x$; use part (e).

####Errata to the digital edition [**](#note2):<a id="title"></a>

The app01.html file was a mess, particulary with the images. Some of them incompletes or just incorrect. Let me know if you find one of my corrections wrong.

  - On id="page\_29":

    - Before: \[...\] is that $∑\_\{R(j)\}∣aj∣$ exists.\]
    - Actual: \[...\] is that $∑\_\{R(j)\}|a\_\{j\}|$ exists.\]

  - On id="page\_29":

    - Before: — that is, if $∑\_\{R(i)\} ∑\_\{S(j)\}∣aj∣$ exists —
    - Actual: — that is, if $∑\_\{R(i)\} ∑\_\{S(j)\}|a\_\{ij\}|$ exists —

  - Answer **5** of **Section 1.2.4**:

    - Before: &lt;em&gt;except&lt;/em&gt; when $1=\\frac12$.
    - Actual: &lt;em&gt;except&lt;/em&gt; when $x\\bmod1=\\frac12$.

  - Answer **6** of **Section 1.2.4**:

    - Before: $\\lfloor\\sqrt\{x\}\\rfloor=n⇔n^\{2\}≤x\\lt(n+1)^\{2\}⇔n^\{2\}≤\\lfloor\{x\}\\rfloor\\lt(n+1)^\{2\}⇔\\lfloor\\sqrt\{x\}\\rfloor=n$
    - Actual: $\\lfloor\\sqrt\{x\}\\rfloor=n⇔n^\{2\}≤x\\lt(n+1)^\{2\}⇔n^\{2\}≤\\lfloor\{x\}\\rfloor\\lt(n+1)^\{2\}⇔\\left\\lfloor\\sqrt\{\\lfloor\{x\}\\rfloor\}\\right\\rfloor=n$

  - Answer **17** of **Section 1.2.7**:

    - Before: By exercise 4.6.2–6, we have $\{p\\brack k\}\\equiv\\delta\_\{kp\}-\\delta\_\{k1\}\\text\{ (modulo \}p)$
    - Actual: By exercise 4.6.2–6, we have $x^\{\\overline p\}\\equiv x^\{p\}-x\\text\{ (modulo \}p)$

  - Answer **21** of **Section 1.2.8**:

    - Before: \[...\] the solution is $(x^\{n+1\}F\_\{n+1\}+x^\{n+2\}F\_\{n-x\})/(x^\{2\}+x-1)$
    - Actual: \[...\] the solution is $(x^\{n+1\}F\_\{n+1\}+x^\{n+2\}F\_\{n\}-x)/(x^\{2\}+x-1)$

  - Answer **36** of **Section 1.2.8**:

    - Before: \[...\] if and only if $\\lfloor(k+1)\\phi^\{-1\}\\rfloor=1$
    - Actual: \[...\] if and only if $\\lfloor(k+1)\\phi^\{-1\}\\rfloor-\\lfloor k\\phi^\{-1\}\\rfloor=1$

  - Answer **37** of **Section 1.2.8**:

    - Before: &lt;em&gt;Proof:&lt;/em&gt; Let $μ$
    - Actual: &lt;em&gt;Proof:&lt;/em&gt; Let $μ(m)=F\_j$;

  - Answer **6** of **Section 1.2.10**:

    - Before: $6\\sqrt\{2\}/5\\approx1.697$
    - Actual: $\\ln(q+pe^\{t\})=\\ln\\left(1+pt+\\frac\{pt^\{2\}\}\{2\}+\\frac\{pt^\{3\}\}\{6\}+\\cdots\\right)=pt+p(1-p)\\frac\{t^\{2\}\}\{2\}+p(1-p)(1-2p)\\frac\{t^\{3\}\}\{6\}+\\cdots$

  - Answer **22** of **Section 1.2.10**:

    - Before: \[...\] it is $1/2$.
    - Actual: \[...\] it is $\\lt 1/2$.

  - Answer **3** of **Section 1.2.11.2**:

    - Before: \[...\] we have $B\_\{m\}(\\frac12)=(2^\{1-m\}-1)$.
    - Actual: \[...\] we have $B\_\{m\}(\\frac12)=(2^\{1-m\}-1)B\_\{m\}$.

  - Answer **8** of **Section 1.2.11.3**:

    - Before: $R(x)=\\int\_\{0\}^\{f(x)\}(e^\{-g(u,x)\}-e^\{-h(u,x)\})$
    - Actual: $R(x)=\\int\_\{0\}^\{f(x)\}(e^\{-g(u,x)\}-e^\{-h(u,x)\})du$

  - Answer **11** of **Section 1.2.11.3**:

    - Before: \[...\] to note that $Q\_\{-1\}(n)=(-1)^\{n\}n!/(e^\{n\}n^\{n\})\\approx(-1)^\{n\}\\sqrt\{2\\pi n\}/e^\{2n\}$
    - Before: \[...\] to note that $R\_\{-1\}(n)-Q\_\{-1\}(n)=(-1)^\{n\}n!/(e^\{n\}n^\{n\})\\approx(-1)^\{n\}\\sqrt\{2\\pi n\}/e^\{2n\}$

  - Answer **37** of **Section 1.2.8**:

    - Before: $μ(n-μ(n))=F\_\{k\_\{r-1\}\}≥F\_\{k\_\{r+2\}\}\\gt 2F\_\{k\_\{r\}\}$
    - Actual: $μ(n-μ(n))=F\_\{k\_\{r-1\}\}≥F\_\{k\_\{r\}+2\}\\gt 2F\_\{k\_\{r\}\}$

  - Answer **41** of **Section 1.2.8**:

    - Before: $\\phihat^\{\\,3\}+\\phihat^\{\\,5\}+\\cdots=\\phihat^\{\\,-1\}$
    - Actual: $\\phihat^\{\\,3\}+\\phihat^\{\\,5\}+\\cdots=\\phihat^\{\\,-1\}-1$

  - Answer **10** of **Section 1.2.9**:

    - Before: **ausent**.
    - Actual: $e\_\{1\}=S\_\{1\}$,

  - Answer **23** of **Section 1.2.9**:

    - Before: $g\_\{2\}(z\_\{1\},z\_\{2\})=z\_\{1\}+z\_\{2\}+z\_\{1\}+z\_\{2\}$
    - Actual: $g\_\{2\}(z\_\{1\},z\_\{2\})=z\_\{1\}+z\_\{2\}+z\_\{1\}z\_\{2\}$

  - On id="page\_172":

    - Before: "We will show below that, if the output permutation is assumed to be random, the quantities &lt;em&gt;U&lt;/em&gt; and &lt;em&gt;υ&lt;/em&gt; will be $H_{N}$ and 1, respectively, on the average."
    - Actual: "We will show below that, if the output permutation is assumed to be random, the quantities &lt;em&gt;U&lt;/em&gt; and &lt;em&gt;V&lt;/em&gt; will be $H_{N}$ and 1, respectively, on the average."

####TODO:

  - Replace &lt;p class="center"&gt;&lt;span class="middle"&gt; for &lt;div class="image"&gt;


<a id="note1"></a>[*](#err1) Found it by chance. That's weird, according to the date Knuth applied the fix, that bug should not be there.
This force me to check all the erratas. Later I will.

<a id="note2"></a>[**](#title) The list does not include all errors I fixed, only those in which I'm not entirely sure if the correction is correct.